Start noodling around

PostComplete/Basic.lean
@@ -1,1 +1,226 @@
-def hello := "world"
+import Mathlib.Data.Fin.VecNotation
+import Mathlib.Data.Finite.Basic
+import Mathlib.Data.FinEnum
+
+#check ![true, true, false, true]
+
+abbrev Func n := (Fin n → Bool) → Bool
+
+#check λ f : Func 2 ↦ f ![true, true]
+
+#check ![]
+
+#print Func
+
+#print Set
+
+def Family := ∀ n : ℕ, Set (Func n)
+
+-- A tree of composition of n inputs, or "vars"
+-- Where each node is a symbolic application of
+-- f ∈ F
+inductive AppTree (F : Family) n :=
+| Var : Fin n → AppTree F n
+| App : ∀ {m} f, f ∈ F m → (Fin m → AppTree F n) → AppTree F n
+
+-- Hey we can eval these!
+def evalTree (t : AppTree F n) : Func n :=
+  λ i ↦
+  match t with
+  | .Var n => i n
+  | .App f _ t => f (λ m ↦ evalTree (t m) i)
+
+#print FinEnum
+
+instance bFinEnum : FinEnum Bool :=
+⟨  2, ⟨ λ b ↦ if b then 1 else 0,
+       λ i ↦ if i.val = 0 then false else true,
+  by
+    simp [Function.LeftInverse]
+  ,
+  by
+    simp [Function.RightInverse, Function.LeftInverse]
+    intros x; split
+    case isTrue h => omega
+    case isFalse h => omega
+⟩
+⟩
+
+instance finEnumFunc n : FinEnum (Func n) := inferInstance
+
+def FuncList (n : ℕ) : List (Func n) :=
+  @FinEnum.toList _ (finEnumFunc n)
+
+@[simp]
+lemma mem_FuncList n : ∀ f, f ∈ FuncList n := by
+  intros f; apply FinEnum.mem_toList
+
+lemma func_to_finite n (P : Func n → Prop) :
+  (∀ f ∈ FuncList n, P f) → ∀ f, P f := by
+  intros p_bound f; apply p_bound; simp
+
+#print FinEnum.toList
+
+#reduce List.length (finEnumFunc 2).toList
+
+-- Are functions extensional?
+lemma test : (λ b ↦ if b then false else true) = not :=
+by
+  apply funext; intro b; split <;> simp at * <;> assumption
+
+-- FIXME: should this be a sigma?
+def CompleteForFN (F G : Family) (n : ℕ) : Prop := ∀ (f : Func n), f ∈ G n → ∃ (t : AppTree F n) , evalTree t = f
+
+def Full : Family := λ _ ↦ Set.univ
+
+def CompleteForN (F : Family) : ℕ → Prop := CompleteForFN F Full
+
+-- Shockingly, this definition does not allow us to do any of the "usual" proofs!
+def Complete F := ∀ n, CompleteForN F n
+
+def QuasiComplete F := ∀ n, n > 0 → CompleteForN F n
+
+def not1 : Func 1 := λ b ↦ ! (b 0)
+
+def true_n : Func n := λ _ ↦ true
+
+def false_n : Func n := λ _ ↦ false
+
+def or2 : Func 2 := λ b ↦ (b 0) || (b 1)
+
+def and2 : Func 2 := λ b ↦ (b 0) && (b 1)
+
+#print Set
+
+@[simp]
+def NotTrueFam : ∀ n, Set (Func n)
+| 0 => ∅
+| 1 => { f | f = not1 ∨ f = true_n }
+| _ => ∅
+
+@[simp]
+def NotAndOrFam : ∀ n, Set (Func n)
+| 0 => ∅
+| 1 => { f | f = not1 }
+| 2 => {f | f = and2 ∨ f = or2 }
+| _ => ∅
+
+#print NotAndOrFam
+
+lemma test' : and2 ∈ NotAndOrFam 2 := by simp
+
+def inst_arg (i : Fin n → Bool)(k : ℕ)(_ : k < n + 1)(b : Bool) : Fin (n+1) → Bool
+| ⟨ l, _⟩ =>
+  if h: l < k then i ⟨ l, by omega⟩
+  else if h': l = k then b
+  else i ⟨ l - 1, by omega⟩
+
+def inst_fun (f : Func (n+1)) (k : ℕ) (h : k < n + 1) (b : Bool) : Func n :=
+  λ arg ↦ f (inst_arg arg k h b)
+
+#print Func
+
+instance subsetFam : HasSubset Family :=
+ ⟨λ F F' ↦ ∀ n, F n ⊆ F' n⟩
+
+def bumpTree {F F'} (sub : F ⊆ F') (t : AppTree F n) : AppTree F' n :=
+match t with
+| .Var n => .Var n
+| .App f _ ts => .App f (by apply sub; trivial) (λ b ↦ bumpTree sub (ts b))
+
+lemma eval_bumpTree_eq  {F F'} (sub : F ⊆ F') (t : AppTree F n) :
+  evalTree t = evalTree (bumpTree sub t) :=
+by
+  cases t
+  case Var n => simp [bumpTree, evalTree]
+  case App =>
+    simp [bumpTree, evalTree]
+    apply funext
+    intros b
+    apply congrArg
+    apply funext
+    intros i;
+    apply congr_fun
+    apply eval_bumpTree_eq
+
+def var_n : Fin n → AppTree F n := λ i ↦ .Var i
+
+@[simp]
+lemma eval_app_eq {F : Family} (f : Func n) (h : f ∈ F n) :
+  evalTree (.App f h var_n) = f := by
+simp [evalTree]
+
+lemma complete_for_n_mon_1 (F F') n : F ⊆ F' → CompleteForN F n → CompleteForN F' n :=
+by
+  simp [CompleteForN, CompleteForFN]
+  intros sub h f _
+  specialize h f _; trivial
+  cases h
+  case intro t eq_t =>
+    exists (bumpTree sub t)
+    rw [← eval_bumpTree_eq]; trivial
+
+
+lemma list_complete {F} (ts : List (AppTree F n)) : False
+/- (same_len : (FuncList n.length) = ts.length) →
+   (∀ k : (Fin (FuncList n).length), evalTree (ts.get k) = (FuncList n).get k) →
+  CompleteForN F n
+ -/
+ := by
+  sorry
+
+#print Family
+
+def EvalMap (F G : Family) : Type := Π {n} f, f ∈ F n → AppTree G n
+
+def EvalMapSound {F G} (e : EvalMap F G) :=
+  ∀ n f (h : f ∈ F n), evalTree (e f (by trivial)) = f
+
+def appTreeSubst {F} (t : AppTree F n) (ts : Fin n → AppTree F m) : AppTree F m :=
+match t with
+| .Var k => ts k
+| .App f mem us =>
+  .App f mem (λ i ↦ appTreeSubst (us i) ts)
+
+#print AppTree
+
+def mapSubst {F G} (e : EvalMap F G) (t : AppTree F n) : AppTree G n :=
+match t with
+| .Var k => .Var k
+| .App f mem ts =>
+    appTreeSubst (e f mem) (λ i ↦ mapSubst e (ts i))
+
+@[simp]
+def mapSubst_sound {F G} (e : EvalMap F G) : EvalMapSound e →
+  ∀ (t : AppTree F n), evalTree (mapSubst e t) = evalTree t
+:= by sorry
+
+lemma eval_mon_complete {F F'} : CompleteForN F' n →
+  (∀ f ∈ F' n, ∃ t : AppTree F n, evalTree t = f) →
+  CompleteForN F n
+:= by sorry
+
+lemma complete_NotTrue_1 : CompleteForN NotTrueFam 1 := by
+  intros f
+  have h_case :
+  (f ![true] = true ∧ f ![false] = true) ∨
+  (f ![true] = false ∧ f ![false] = true) ∨
+  (f ![true] = false ∧ f ![false] = false) ∨
+  (f ![true] = true ∧ f ![false] = false) := by
+    sorry
+  cases h_case
+  case inl h => sorry
+  case inr h => sorry
+
+
+theorem complete_NotAndOrFam : QuasiComplete NotAndOrFam :=
+by
+  intros n
+  cases n
+  case zero => intros _ h; omega
+  case succ n =>
+    intros _ f
+    let f_true : Func n := inst_fun f n (by simp) true
+    let f_false : Func n := inst_fun f n (by simp) false
+    let tree_f := complete_NotAndOrFam _ _ f_true
+    sorry
